---
id: 1759330574-MWHI
aliases:
  - 2nd Order - Reduction of Order
tags: []
---

# 2nd Order - Reduction of Order
# Reduction of Order (3.3) 

## Application Scenarios
If $y_1$ is a solution of the homogenous equation; *can it help us to find $y_2$?*

Remark: recall from algebra the example
* If $x=1$ is root of $x^3-7x+6=0$ 
* Then we can use division of polynomials to simplify the problem 

In differential equations, we will consider $y_2=v(x)y_1$ note $v(x)$ **must not be a constant** for linear indepdence to hold true

Thus, the question is how can we find $v(x)$? Simply use the application of **Reduction of Order**

This takes a second-order equation into a first-order equation.

## Application 

We wish to solve (homogenous second order equation): 
$$y''+p(x)y'+q(x)y = 0$$

Using: $y = v(x)y_1$, where $y_1$ solves the homogenous equation 

Therefore, we must find $v(x)$

Taking the derrivatives of $y$ we get the following: 
$$y'=v'(x)y_1 + v(x)y_1'$$
$$y''=v''y_1 + v'y_1' + v'y_1' + vy_1''$$
$$y''=v''y_1 + 2v'y_1' + vy_1''$$

Subsituting into the homogenous equation we get the following:  

$$(v''y_1+2v'y_1'+vy_1'')+p[v'y_1 + vy_1']+qvy_1 = 0$$
* (stuff) is y'' and [stuff] is y'

Let's rearrange this equation, knowing y_1 satisfied the differential equation
$$v(y_1''+py_1'+qy_1) + v'(2y_1'+py_1) + v''y_1 = 0$$

Observe $(y_1''+py_1'+qy_1)$ looks at lot like the homogenous equation, which we know for $y_1$, equals 0. 

Therefore:
$$=v(0) + v'(2y_1'+py_1) + v''y_1 = 0$$
$$= v'(2y_1'+py_1) + v''y_1 = 0$$
$$= v'(2+\dfrac{py_1}{y_1}) + v''= 0$$
Notice this looks at lot like a first order ODE

$$w' + (p+2\dfrac{y_1'}{y_1})w=0$$

### Example

**Problem**: Given a solution $y_1 = e^{3x}$ of $y''-6y'+9y=0$ we want to find a second lineary independent solution and the general solution.

**Solution**:

Suppose $y=v(x)y_1$, let $v(x) = v$ for the sake of brevity

$$y' = v'e^{3x} + 3ve^{3x}$$
$$y'' =  v''e^{3x} + 3v'e^{3x} + 3v'e^{3x} + 9ve^{3x} $$
$$y'' =  v''e^{3x} + 6v'e^{3x} + 9ve^{3x} $$

Subsituting: 

$$(v''e^{3x} + 6v'e^{3x} + 9ve^{3x}) + p(v'e^{3x} + 3ve^{3x}) + qvy = 0$$
$$v''e^{3x} + 6v'e^{3x} + 9ve^{3x} - 6v'e^{3x} - 18ve^{3x} + 9ve^{3x} = 0$$
$$v''e^{3x}= 0$$

*divide both sides by $\dfrac{1}{e^{3x}}$*

$$v''=0$$

Let $w=v'$ s.t. $w'=0$

Thus: $w=$some constant; and $v'=c$

$$v = \int c ~dx = cx + d$$

Since we want only one solution as simple as possible

The general solution $c_1y_1 + c_2y_2 = 0$ where $y_1=e^{3x}$ and $y_2 = v(x)y_1 = v(x)e^{3x}$
* Notice we proposed $v = \int c ~dx = cx + d$.
* Set d=0 and keep c=1 to get $v = \int c ~dx = x$
* $\therefore y_2 = xe^{3x}$
* The general solution is then: $c_1y_2 + c_2y_2 = c_1e^{3x} + c_2xe^{3x}$

### Example: Non-constant coefficents

Given solution $y_1 = e^x$ of $xy''-(2x+1)y'+(x+1)y = 0$ on any interval not containing the origin, find $y_2$ and the general solution

$y_1 = e^x$ 

$xy''-(2x+1)y'+(x+1)y = 0$ 

Let $y=vy_1 = ve^x$
$$ y = ve^x$$
$$ y' = v'e^x + ve^x$$
$$ y'' = v''e^x + v'e^x + v'e^x + ve^x$$
$$ y'' = v''e^x + 2v'e^x + ve^x$$

Subsituting...
$$x[v''e^x+2v'e^x+ve^x ] - (2x+1)[v'e^x+ve^x] + (x+1)ve^x = 0$$

Simplify so that the v terms drop out

$$xv''e^x-v'e^x=0$$

Isolate $v''$

$$v''-\dfrac{1}{x}v'=0$$

Rewrite into 1'st order ODE
$$w'-\dfrac{1}{x}w=0$$

$$w'=\dfrac{1}{x}w$$
$$\dfrac{dw}{dx}=\dfrac{1}{x}w$$
$$\dfrac{1}{w}~dw=\dfrac{1}{x}~dx$$
$$\int \dfrac{1}{w}~dw=\int \dfrac{1}{x}~dx$$
$$ln|w| = ln|x| + C$$
$$e^{ln|w|} = e^{ln|x| + C}$$
$$|w| = |x|e^C$$
$$w = x C$$

Subsequently: 
$$v'-w = Cx$$
$$v = \int Cx = C\dfrac{x^2}{2} + 1$$
Set C = 2, d = 0, s.t. $v = x^2$

## How Equation with Constant Coefficents (Real Roots)

How do real roots relate to the solution?

We wish to solve $ay'' + by' + cy = 0$ 

A good candidate for a solution is: $y(x)=e^{rx}, r \in \mathbb{R}$

To see this consider: 
* $y' = re^{rx}$
* $y'' = r^2e^{rx}$

Subsituting 
$$ g(x) = e^{rx}[ar^2 + rb + c] = 0$$

Observe $e^{rx} \neq 0$ if $g(x)=0$ then this implies there must be two solutions given the quadratic equation $ar^2+rb+c=0$

### Characterisitc Equation
This is called the Characterisitc Equation

The roots for this example are: 

$$r_{1,2} = \dfrac{-b +/- \sqrt{b^2-4ac}}{2a}$$

$$D = b^2 -4ac$$

In general:
* If $D > 0$ then there are two distinct real roots
* If $D = 0$ then there are real roots with multiplicity 2
* If $D < 0$ then are 2 complex conjugate roots


