---
id: "2025-10-20"
aliases: []
tags: []
---

# Variation of Parameters

Consider:
$$y''+p(x)y'+q(x)y=f(x)$$
Observe we have non-constant coefficents

We will search for $y_p = v_1(x)y_1 + v_2(x)y_2$

Where $y_1,y_2$ are the given solution from homogenous equation

Recall we know how to find $y_2$ given $y_1$ using reduction of order

---

* $y_p = v_1y_1 + v_2y_2$
* $y_p' = v_1'y_1 + v_1y_1' + v_2'y_2 + v_2y_2' = (v_1'y_1 + v_2'y_2) + v_1y_1' + v_2y_2'$
    * Note we can set $v_1'y_1 + v_2'y_2$ to zero.

* $y_p' = (0) + v_1y_1' + v_2y_2'$
* $y_p' = v_1y_1' + v_2y_2'$
* $\implies y_p'' = v_1y_1'' + v_1'y_1' + v_2y_2'' + v_2'y_2'$
* $y_p'' = v_1'y_1' + v_2'y_2' + v_1y_1'' + v_2y_2''$
* Subsituting into $y''+p(x)y'+q(x)y=f(x)$ we get the following:
    * $[v_1'y_1' + v_2'y_2' + v_1y_1'' + v_2y_2''] + p[v_1y_1' + v_2y_2'] + q[ v_1y_1 + v_2y_2] = f(x)$
* Recall $y_1,y_2$ are solutions to the homogenous equations
    * $y_1'' + py_1' + qy = 0$
        * $\implies v_1[y_1'' + py_1' + qy] = 0*v_1$
    * $y_2'' + py_2' + qy = 0$
        * $\implies v_2[y_2'' + py_2' + qy] = 0*v_2$
        *  $v_1[y_1'' + py_1' + qy] = 0*v_1 v_2[y_2'' + py_2' + qy] = 0*v_2$
* Observe $[v_1'y_1' + v_2'y_2' + (v_1y_1'' + v_2y_2''] + p[v_1y_1' + v_2y_2'] + q[ v_1y_1 + v_2y_2]) = f(x)$
    * Observe $[v_1y_1'' + v_2y_2''] + p[v_1y_1' + v_2y_2'] + q[ v_1y_1 + v_2y_2]$
        * $= v_1[y_1'' + py_1' + qy] + v_2[y_2'' + py_2' + qy] = 0$

* The parameters $v_1,v_2$ need to satisfy the condititons:
    * $v_1'y_1 + v_2'y_2 = 0$
    * $v_1'y_1' + v_2'y_2' = f(x)$
* Set as matrix:
$$\begin{bmatrix}
y_1 & y_2 \\ 
y_1' & y_2'
\end{bmatrix}
\begin{bmatrix}
v_1' \\ 
v_2' \\
\end{bmatrix} =
\begin{bmatrix}
0 \\
f
\end{bmatrix}
$$
* Solve using Cramer's Rule
* Consider the following: 
    * $a_1x + b_1y = c_1$
    * $a_2x + b_2y = c_2$
$$\begin{bmatrix}
a_1 & b_2 \\ 
a_2 & b_2
\end{bmatrix}
\begin{bmatrix}
x \\ 
y \\
\end{bmatrix} =
\begin{bmatrix}
c_1 \\
c_2
\end{bmatrix}
$$

$$\begin{bmatrix}
a_1*x & b_2*y \\ 
a_2*x & b_2*y
\end{bmatrix} = 
\begin{bmatrix}
c_1 \\
c_2
\end{bmatrix}
$$

Now compute the determinant
$$
D = 
\begin{bmatrix}
a_1 & b_1 \\ 
a_2 & b_2
\end{bmatrix} = a_1b_2 - a_2b_1
$$

$$
D_x = 
\begin{bmatrix}
c_1 & b_1 \\ 
c_2 & b_2
\end{bmatrix} = c_1b_2 - c_2b_1
$$

$$
D_y = 
\begin{bmatrix}
a_1 & c_1 \\ 
a_2 & c_2
\end{bmatrix} = a_1c_2 - a_2c_1
$$

By Cramer's rule the solution of the system is:

$$x=\dfrac{D_x}{D}, y=\dfrac{D_y}{D}$$

In our context: 

$$
D = 
\begin{bmatrix}
y_1 & y_2 \\ 
y_1' & y_2'
\end{bmatrix}
$$

$$
D_x = 
\begin{bmatrix}
0 & y_2 \\ 
f & y_2'
\end{bmatrix} = y_2f
$$

$$
D = 
\begin{bmatrix}
y_1 & 0 \\ 
y_1' & f
\end{bmatrix} = y_1f
$$

---
Just remember this:
$$\implies v_1 = \int\dfrac{Dv_1'}{W} dx = \int\dfrac{-y_2f}{W}dx$$
$$\implies v_2 = \int\dfrac{Dv_2'}{W} dx = \int\dfrac{y_1f}{W}dx$$

## Example w/ Constant Coefficents

Find the general solution
* $y''-y = 5e^x$
* Characterisitic Equation: $r^2-1 = 0$
    * $r_{1,2} = \pm 1$
* $\implies y_h = c_1e^x + c_2e^{-x}$
* Solving for $y_p = v_1y_1 + v_2y_2$ find $v_1,v_2$
$$
W = 
\begin{bmatrix}
y_1 & y_2 \\
y_1' & y_2'
\end{bmatrix} = -2
\begin{bmatrix}
e^x & e^{-x}\\
e^x & -e^{-x}
\end{bmatrix}
$$

$$D_{v_1'} = -y_2f = -e^{-x}5e^x $$
$$D_{v_2'} = y_1f = e^x5e^x$$

$$\implies v_1 = \int{\dfrac{Dv_1'}{W}dx} = \int\dfrac{-e^{-x}5e^x}{-2} = \dfrac{2}{5}\int{e^{-x}e^x} = \dfrac{2}{5}\int{1} = x\dfrac{2}{5} + C_1$$

$$\implies v_2 = \int{\dfrac{Dv_2'}{W}dx = \int\dfrac{e^x5e^x}{-2}} = -\dfrac{5}{2}\int{e^{2x}} = -\dfrac{5}{4}e^{2x} + C_2$$

$$\therefore y =c_1e^x + c_2e^{-x} + \dfrac{5}{2}xe^x + (-\dfrac{5}{4})e^{-x}$$


## Example 
$$y''+y = 1$$

Solution:
$$r^2 +1 = 0 \implies r_{1,2} = \pm i$$
$$y_h = c_1cos(x) + c_2sin(x)$$
Recall
$$y_p = v_1y_1 + v_2y_2$$
$$
W = 
\begin{bmatrix}
y_1 & y_2 \\
y_1' & y_2'
\end{bmatrix} = -2
\begin{bmatrix}
cos(x) & sin(x)\\
-sin(x) & cos(x)
\end{bmatrix} = cos^2(x) + sin^2(x) = 1
$$


$$D_{v_1'} = -y_2f = -sin(x)(1) $$
$$D_{v_2'} = y_1f = cos(x)$$
