---
id: "2025-10-01"
aliases: []
tags: []
---

# Table of Contents 

# Recall 

Recall 2nd order DEs with constant coeff homo

$$ay''+ by' + cy = 0 $$

Candidate Solution $y = e^{rx}, y''=re^{rx}, y'' r^2e^{rx}$ 

Subsituting Gives: 

$$e^{rx}(ar^2 + r + c) = 0, \text{since } e^{rx} \neq 0$$

Provides the characteristic equation: $ar^2 + br + c = 0$

$$r_{1,2} = \dfrac{-b \pm \sqrt{b^2-4ac}}{2a}$$


$$D = b^2 -4ac$$

In general:
* If $D > 0$ then there are two distinct real roots
* If $D = 0$ then there are real roots with multiplicity 2
* If $D < 0$ then are 2 complex conjugate roots

$$y = c_1y_1 + c_2y_2 =  c_1e^{r_1x} + c_2e^{r_2x}$$

## Example IVP:

$$y(0)=1, y''-y = 0, y'(0)=0$$


### Write Characteristic Equation 

Given from $ay''+ by' + cy = 0 $, (a,b,c)

$$r^2-1 = 0$$

Plug in $r_1$, $r_2$ which is $\pm 1$

$$y = c_1e^{-x} + c_2e^{x}$$

Solving IVP: 

$$y = c_1e^{-x} + c_2e^{x}$$
$$y' = -c_1e^{-x} + c_2e^{x}$$

Plug in ini. conditions. 


$$y = c_1e^{-x} + c_2e^{x} = 1$$
$$\therefore c_1 + c_2 = 1$$


$$y' = -c_1e^{-x} + c_2e^{x} = 0$$
$$\therefore -c_1 + c_2 = 0 $$

Combine equations
$$\therefore -c_1 + c_2 = 0 $$
$$\therefore c_1 + c_2 = 1$$
$$\therefore  2c_2 = 1$$
$$\therefore  c_2 = 1/2 = c_1$$


## Case 2:

D=0 characteristic equation has 1 real root of multiplicity 2 and the general solution of $ay''+ by' + cy = 0$ is the following:

$$y = c_1y_1 + c_2y_2 =  c_1e^{rx} + c_2e^{rx}$$

Apply reduction of order to remove linear dependency

$$y = c_1y_1 + c_2y_2 =  c_1e^{rx} + c_2xe^{rx}$$

Example: Find the general solution of $y''+4y'+4y=0$

### Write Characteristic Equation

$r^2 + 4r + 4 = 0$

$(r+2)^2 = 0$

This imples the root $r_{1,2} = -2$

Therefore: 
* $y_1 = e^{-2x}$
* $y_2 = xe^{-2x}$

$$y=c_1y_1 + c_1y_2 = c_1e^{-2} + c_2xe{^-2x}$$

## Case 3: 
D < 0, the roots of the characteristic equation is a complex conjugate pair.

$$r_{1,2} = \dfrac{-b \pm \sqrt{b^2-4ac}}{2a} = \dfrac{-b \pm i\sqrt{-b^2+4ac}}{2a} = -\dfrac{b}{2a} \pm i\dfrac{\sqrt{4ac-b^2}}{2a}$$
$$ = p \pm iq$$
$$ p = -\dfrac{b}{2a}, q = \pm \dfrac{\sqrt{4ac-b^2}}{2a}$$

## Recall Euler's Formula 

If x is any number then:
$$e^{ix}= cos(x) + isin(x)$$

$$e^{i\pi} + 1 = 0$$
$$e^{2\pi i } = 1$$

### Proof From Taylor's Expansion: 

$$f(x) = e^x \text{about} x_0 = 0$$

Then we have the following: 

$$e^x = 1 + x + \dfrac{x^2}{2!} + \dfrac{x^3}{3!} + ... + \dfrac{x^n}{n!} + \dfrac{x^{n+1}}{(n+1)!} e^{\xi_x}$$

$$\xi_x \in [0,x]$$

So for $f(x) = e^{ix}$, we get: 

$$e^x = 1 + x + \dfrac{x^2}{2!} + \dfrac{x^3}{3!} + ... + \dfrac{x^n}{n!} + \dfrac{x^{n+1}}{(n+1)!} e^{\xi_x}$$

$$e^x = 1 - \dfrac{x^2}{2!} + \dfrac{x^4}{4!} - \dfrac{x^6}{6!} + ...$$
$$...+ i(x - \dfrac{x^3}{3!} + \dfrac{x^5}{5!} + ...)$$

Observe: 
$$cos(x) = e^x = 1 - \dfrac{x^2}{2!} + \dfrac{x^4}{4!} - \dfrac{x^6}{6!} + ...$$
$$sin(x) = i(x - \dfrac{x^3}{3!} + \dfrac{x^5}{5!} + ...)$$

Observe a special case: 
$$e^{-ix} = e^{i(-x)} = cos(-x) + isin(-x) = cos(x) - isin(x)$$

## Using the Euler's Formula: General Solution

$$y = c_1y_1 + c_2y_2 = c_1e^{r_1x} +c_2e^{r_2x}$$

Recall $r_{1,2} = p \pm iq$

$$y = c_1y_1 + c_2y_2 = c_1e^{(p + iq)x} +c_2e^{(p - iq)x}$$

$$y = c_1e^{px}e^{iqx} + c_2e^{px}e^{-iqx}$$
$$=c_1e^{px}[cos(qx) + isin(qx)] + c_2e^{px}[cos(qx)-isin(qx)]$$
$$=(c_1+c_2)e^{px}cos(qx)+i(c_1-c_2)e^{px}sin(qx)$$
$$=C_1e^{px}cos(qx)+C_2e^{px}sin(qx)$$

Therefore: 

$$y = C_1e^{px}cos(qx)+C_2e^{px}sin(qx)$$

Remark: In general constants and the solutions can be complex but if we search for real solutions we use real constants

# Example Find the General Solution of: 
$$y'' + 2y' + 4y = 0$$

Solution Characteristic Equation is: 

$$r^2 + 2r +  4 = 0$$

$$r_{1,2} = \dfrac{-2 \pm \sqrt{4-16}}{2} = \dfrac{-2 \pm i \sqrt{12}}{2} = -1 \pm \sqrt{3}$$

Therefore the general solution is: 

$$y = c_1y_2 + c_2y_2 = c_1e^{-x}cos(i\sqrt{3}x) + c_2 e^{-x}sin(\sqrt{3}x)$$

# Example IVP 

$$y''+4y=0, y(0)=1, y'(0)=-1$$

Characteristic Equation: 
$$r^2 + 4 = 0$$

$$r_{1,2} = \pm 2i$$

General Solution

$$y=c_1y_1 + c_2y_2 = c_1cos(2x) + c_2sin(2x)$$

# Example IVP

$$y' = 2c_1sin(2x) + 2c_2cos(2x), y(0)=1$$
$$y=c_1y_1 + c_2y_2 = c_1cos(2x) + c_2sin(2x)$$

$$1 = c_1 + c_2 * 0$$
$$-1 = -2c_1 * 0 + 2c_2$$

$$c_1 = 1, c_2 = -0.5$$
