---
id: "2025-10-06"
aliases: []
tags: []
---

# Table of Contents 

<!-- vim-markdown-toc GFM -->

* [Solving 2nd Order ODE's with Non-Zero RHS](#solving-2nd-order-odes-with-non-zero-rhs)
    * [How can we find $y_p$?](#how-can-we-find-y_p)
        * [Example](#example)
    * [Principle of Superposition](#principle-of-superposition)
    * [Example:](#example-1)

<!-- vim-markdown-toc -->
# Solving 2nd Order ODE's with Non-Zero RHS
Consider: 
$$ay''+bp(x)y'+cq(x)y = f(x) a,b,c \in \mathbb{R}$$
Solution: 
$$y_h + y_p = f(x)$$
Where: 
* $y_h$ is the solution to the homogenous equation 
* $y_p$ is the particular solution - any solution for the given RHS=f(x)


$$[c_1y_1 + c_2y_2] + y_p = f(x), y_1 \ne zy_2, z \in \mathbb{R}$$

## How can we find $y_p$?
* Simple idea is to use 'educated guess'

### Example 
Solve:
$$y''+y=1$$
Solution:

We need to find both $y_h$ and $y_p$

1. Form Characteristic Equation
$$r^2 + 1 = 0 \implies r = \pm i$$
$$p = 0, q = 1$$
$$y_h = c_1e^{px}cosqx + c_2e^{px}sinqx = c_1cosx + c_2sinx$$

By inspection we try $y_p = 1$:
$$y = y_h + y_o + c_1cosx + c_2sinx + 1$$

## Principle of Superposition
Question: What can we do if f(x) is more general?

Principle of Superposition is useful when $f(x) = f_1(x) + f_2(x) + ... + f_n(x)$

By finidng the solution to each $f_n(x)$ term we can sum all the terms to find the f(x)

For example: $f(x) = 1 + cos(4x)$

1. Scalar Property 
* If $y$ is a solution of $y'' + py' + qy = f(x)$; then $ky \_ = kf(X)$

2. Additive Property
* If $y_1$ is a solution of: $\_ = f_1(x)$
* If $y_2$ is a solution of: $\_ = f_2(x)$
* Then $y_1 + y_2$ is a solution of: $\_ = f_1(x) + f_2(x)$

Remark: $y_1$ and $y_2$ can be combined to find the solution of $\sum f_1(x) + f_2(x)$
Remark: We can look at DE as input/output systems
                                                                  
```
external force           system           response of the system               
    f(x)            $y'' +py' + qy$               y                
                                                   
```

In other words if we scale the input, the output gets scaled in the same way

If input is $c_1f_1 + c_2f_2$ then the output is $c_1y_1 + c_2y_2$


## Example: 

if $y''+y'+2y = x$ has a solution $y_1(x) = 0.5x-1$

Also, $y''+y'+2y = e^x$ has a solution $y_2(x)=0.25e^x$

And we wanted to find a solution to: 

$$y'' + y' + 2y = 5x + 3e^x$$

Solution: 

$5f_1 + 3f_2$ so the solution must be $y = 5y_1 + 3y_2 = 5(0.5x-1) + 3(0.25)e^x$
